

H CORRECTED PRIVACY BUDGET BOUNDS IN LATENT [5]

In this section, we aim at providing corrected privacy budget bounds for LATENT [5]. LATENT first encodes embedded features e into an dl -bit bit-string B . Then, each bit $j \in [0, dl - 1]$ is randomized by a RR mechanism (i.e., the MOUE algorithm for high sensitivities in Theorem 3.3 [5]), denoted f -LT, as follows:

$$\forall j \in [0, dl - 1] : P(\tilde{B}_j = 1) = \begin{cases} p_j = \frac{1}{1 + \alpha}, & \text{if } B_j = 1 \\ q_j = \frac{1}{1 + \alpha \exp(\frac{\epsilon_f}{dl})}, & \text{if } B_j = 0 \end{cases} \quad (30)$$

From Eq. 30, we also have that $P(\tilde{B}_j = 0) = 1 - p_j = \frac{\alpha}{1 + \alpha}$ if $B_j = 1$, and $P(\tilde{B}_j = 0) = 1 - q_j = \frac{\alpha \exp(\frac{\epsilon_f}{dl})}{1 + \alpha \exp(\frac{\epsilon_f}{dl})}$ if $B_j = 0$.

Theorem 8. LATENT with the randomization probabilities as in Eq. 30 preserves $\epsilon_{corrected}$ -LDP, where $\epsilon_{corrected} = \frac{(1 + \alpha)(1 + \alpha \exp(\frac{\epsilon_f}{dl}))}{\alpha(1 + \exp(\frac{\epsilon_f}{dl}))} \epsilon_f$.

PROOF. Similar to the analysis in **Appx.F**, we obtain the following inequality:

$$\frac{P(f\text{-LT}(B) = \tilde{B})}{P(f\text{-LT}(B') = \tilde{B})} \leq \prod_{j=0}^{dl-1} \left(\frac{P(f\text{-LT}(B_j) = \tilde{B}_j)}{P(f\text{-LT}(B'_j) = \tilde{B}_j)} \right)^{\frac{\Delta_j}{\mathbb{E}|\mathcal{R}(f\text{-LT}(B, j)) - \mathcal{R}(f\text{-LT}(B', j))|}} \leq \exp(\epsilon_f) \quad (31)$$

and the expectation $\mathbb{E}|\mathcal{R}(f\text{-LT}(B, j)) - \mathcal{R}(f\text{-LT}(B', j))|$ is computed as follows:

$$\begin{aligned} & \mathbb{E}|\mathcal{R}(f\text{-LT}(B, j)) - \mathcal{R}(f\text{-LT}(B', j))| \\ &= \left(P(f\text{-LT}(B_j) = 1 | B_j = 1) P(f\text{-LT}(B'_j) = 0 | B'_j = 0) P(B'_j = 0) \right. \\ & \quad \left. + P(f\text{-LT}(B_j) = 1 | B_j = 0) P(f\text{-LT}(B'_j) = 0 | B'_j = 1) P(B'_j = 1) \right) \Delta_j \\ & \quad + \left(P(f\text{-LT}(B_j) = 0 | B_j = 1) P(f\text{-LT}(B'_j) = 1 | B'_j = 0) P(B'_j = 0) \right. \\ & \quad \left. + P(f\text{-LT}(B, j) = 0 | B_j = 0) P(f\text{-LT}(B'_j) = 1 | B'_j = 1) P(B'_j = 1) \right) \Delta_j \\ &= \left(p_j(1 - q_j) P(B'_j = 0) + q_j(1 - p_j) P(B'_j = 1) + (1 - p_j) q_j P(B'_j = 0) + (1 - q_j) p_j P(B'_j = 1) \right) \Delta_j \\ &= \left(p_j(1 - q_j) + q_j(1 - p_j) \right) \Delta_j \end{aligned} \quad (32)$$

Furthermore, we have:

$$p_j(1 - q_j) + q_j(1 - p_j) = \frac{\alpha(1 + \exp(\frac{\epsilon_f}{dl}))}{(1 + \alpha)(1 + \alpha \exp(\frac{\epsilon_f}{dl}))} \quad (33)$$

From Eqs. 31-33, we have that

$$\begin{aligned} & \frac{P(f\text{-LT}(B) = \tilde{B})}{P(f\text{-LT}(B') = \tilde{B})} \leq \prod_{j=0}^{dl-1} \left(\frac{P(f\text{-LT}(B_j) = \tilde{B}_j)}{P(f\text{-LT}(B'_j) = \tilde{B}_j)} \right)^{\frac{\Delta_j}{\mathbb{E}|\mathcal{R}(f\text{-LT}(B, j)) - \mathcal{R}(f\text{-LT}(B', j))|}} \\ &= \prod_{j=0}^{dl-1} \left(\frac{P(f\text{-LT}(B_j) = 1 | B_j = 1)}{P(f\text{-LT}(B_j) = 0 | B_j = 1)} \right)^{\frac{\Delta_j}{(p_j(1 - q_j) + q_j(1 - p_j)) \Delta_j}} \times \prod_{j=0}^{dl-1} \left(\frac{P(f\text{-LT}(B_j) = 0 | B_j = 0)}{P(f\text{-LT}(B_j) = 1 | B_j = 0)} \right)^{\frac{\Delta_j}{(p_j(1 - q_j) + q_j(1 - p_j)) \Delta_j}} \\ &= \prod_{j=0}^{dl-1} \left(\exp(\frac{\epsilon_f}{dl}) \right)^{\frac{1}{p_j(1 - q_j) + q_j(1 - p_j)}} \end{aligned} \quad (34)$$

Then, from Eq. 34, we have:

$$\epsilon_{corrected} = \ln \left(\prod_{j=0}^{dl-1} \left(\exp(\frac{\epsilon_f}{dl}) \right)^{\frac{1}{p_j(1 - q_j) + q_j(1 - p_j)}} \right) = \frac{(1 + \alpha)(1 + \alpha \exp(\frac{\epsilon_f}{dl}))}{\alpha(1 + \exp(\frac{\epsilon_f}{dl}))} \epsilon_f \quad (35)$$

Consequently, Theorem 8 holds. \square

I CORRECTED PRIVACY BUDGET BOUNDS IN OME [29]

In this section, we aim at providing corrected privacy budget bounds for OME. OME first encodes the embedding features z into an dl -bit binary vector B . Then, each bit $j \in [0, dl - 1]$ is randomized by the following f -OME mechanism:

$$\forall j \in [0, dl - 1] : P(\tilde{B}_j = 1) = \begin{cases} p_{1j} = \frac{\alpha}{1 + \alpha}, & \text{if } j \in 2k, B_j = 1 \\ p_{2j} = \frac{1}{1 + \alpha^3}, & \text{if } j \in 2k + 1, B_j = 1 \\ q_j = \frac{1}{1 + \alpha \exp(\frac{\epsilon_f}{dl})}, & \text{if } B_j = 0 \end{cases} \quad (36)$$

From Eq. 36, we also have that $P(\tilde{B}_j = 0) = 1 - p_{1j} = \frac{1}{1 + \alpha}$ if $B_j = 1$ and $j \in 2k$, $P(\tilde{B}_j = 0) = 1 - p_{2j} = \frac{\alpha^3}{1 + \alpha^3}$ if $B_j = 1$ and $j \in 2k + 1$, and $P(\tilde{B}_j = 0) = 1 - q_j = \frac{\alpha \exp(\frac{\epsilon_f}{dl})}{1 + \alpha \exp(\frac{\epsilon_f}{dl})}$ if $B_j = 0$.

Theorem 9. *OME with the randomization probabilities as in Eq. 36 preserves $\epsilon_{corrected}$ -LDP, where $\epsilon_{corrected} = (\frac{dl}{Q_1} - \frac{dl}{Q_2}) \ln(\alpha) + \frac{\epsilon_f}{2Q_1} + \frac{\epsilon_f}{2Q_2}$ in which $Q_1 = \frac{\alpha}{1 + \alpha} \frac{\alpha \exp(\frac{\epsilon_f}{dl})}{1 + \alpha \exp(\frac{\epsilon_f}{dl})} + \frac{1}{1 + \alpha \exp(\frac{\epsilon_f}{dl})} \frac{1}{1 + \alpha}$ and $Q_2 = \frac{1}{1 + \alpha^3} \frac{\alpha \exp(\frac{\epsilon_f}{dl})}{1 + \alpha \exp(\frac{\epsilon_f}{dl})} + \frac{1}{1 + \alpha \exp(\frac{\epsilon_f}{dl})} \frac{\alpha^3}{1 + \alpha^3}$.*

PROOF. Similar to the analysis in **Appx. F** and **Appx. H**, we obtain:

$$\frac{P(f\text{-OME}(B) = \tilde{B})}{P(f\text{-OME}(B') = \tilde{B})} \leq \prod_{j=0}^{dl-1} \left(\frac{P(f\text{-OME}(B_j) = \tilde{B}_j)}{P(f\text{-OME}(B'_j) = \tilde{B}_j)} \right)^{\frac{\Delta_j}{\mathbb{E}|\mathcal{R}(f\text{-OME}(B, j)) - \mathcal{R}(f\text{-OME}(B', j))|}} \leq \exp(\epsilon_f) \quad (37)$$

and the expectation $\mathbb{E}|\mathcal{R}(f\text{-OME}(B, j)) - \mathcal{R}(f\text{-OME}(B', j))|$ is computed as follows:

$$\mathbb{E}|\mathcal{R}(f\text{-OME}(B, j)) - \mathcal{R}(f\text{-OME}(B', j))| = \begin{cases} (p_{1j}(1 - q_j) + q_j(1 - p_{1j}))\Delta_j = Q_1\Delta_j, & \text{if } j \in 2k \\ (p_{2j}(1 - q_j) + q_j(1 - p_{2j}))\Delta_j = Q_2\Delta_j, & \text{if } j \in 2k + 1 \end{cases} \quad (38)$$

where $Q_1 = p_{1j}(1 - q_j) + q_j(1 - p_{1j}) = \frac{\alpha}{1 + \alpha} \frac{\alpha \exp(\frac{\epsilon_f}{dl})}{1 + \alpha \exp(\frac{\epsilon_f}{dl})} + \frac{1}{1 + \alpha \exp(\frac{\epsilon_f}{dl})} \frac{1}{1 + \alpha}$, and $Q_2 = p_{2j}(1 - q_j) + q_j(1 - p_{2j}) = \frac{1}{1 + \alpha^3} \frac{\alpha \exp(\frac{\epsilon_f}{dl})}{1 + \alpha \exp(\frac{\epsilon_f}{dl})} + \frac{1}{1 + \alpha \exp(\frac{\epsilon_f}{dl})} \frac{\alpha^3}{1 + \alpha^3}$.

From Eqs. 37 and 38, we have:

$$\begin{aligned} \frac{P(f\text{-OME}(B) = \tilde{B})}{P(f\text{-OME}(B') = \tilde{B})} &\leq \prod_{j=0}^{dl-1} \left(\frac{P(f\text{-OME}(B_j) = \tilde{B}_j)}{P(f\text{-OME}(B'_j) = \tilde{B}_j)} \right)^{\frac{\Delta_j}{\mathbb{E}|\mathcal{R}(f\text{-OME}(B, j)) - \mathcal{R}(f\text{-OME}(B', j))|}} \\ &= \prod_{j \in 2k} \left(\frac{P(f\text{-OME}(B_j) = 1|B_j = 1)P(f\text{-OME}(B_j) = 0|B_j = 0)}{P(f\text{-OME}(B_j) = 1|B_j = 0)P(f\text{-OME}(B_j) = 0|B_j = 1)} \right)^{\frac{\Delta_j}{Q_1\Delta_j}} \\ &\quad \times \prod_{j \in 2k+1} \left(\frac{P(f\text{-OME}(B_j) = 1|B_j = 1)P(f\text{-OME}(B_j) = 0|B_j = 0)}{P(f\text{-OME}(B_j) = 1|B_j = 0)P(f\text{-OME}(B_j) = 0|B_j = 1)} \right)^{\frac{\Delta_j}{Q_2\Delta_j}} \\ &= \alpha^{\frac{dl}{Q_1} - \frac{dl}{Q_2}} \exp\left(\frac{\epsilon_f}{2Q_1} + \frac{\epsilon_f}{2Q_2}\right) \end{aligned} \quad (39)$$

Then, from Eq. 39, we have:

$$\epsilon_{corrected} = \ln \left(\alpha^{\frac{dl}{Q_1} - \frac{dl}{Q_2}} \exp\left(\frac{\epsilon_f}{2Q_1} + \frac{\epsilon_f}{2Q_2}\right) \right) \quad (40)$$

$$= \left(\frac{dl}{Q_1} - \frac{dl}{Q_2} \right) \ln(\alpha) + \frac{\epsilon_f}{2Q_1} + \frac{\epsilon_f}{2Q_2} \quad (41)$$

Consequently, Theorem 9 does hold. \square